The new verifier code is almost nearing completion

LinearScan.hs
@@ -29,21 +29,21 @@ import qualified Data.IntMap as M
 import           Data.IntSet (IntSet)
 import qualified Data.IntSet as S
 import qualified Data.List as L
+import           Data.Maybe (fromMaybe)
 import           Debug.Trace
 import qualified Hask.Utils as LS
 import qualified LinearScan.Applicative as Coq
-import qualified LinearScan.Blocks as LS
 import           LinearScan.Blocks
+import qualified LinearScan.Blocks as LS
 import qualified LinearScan.Functor as Coq
 import qualified LinearScan.Functor as Functor
-import qualified LinearScan.IntMap as LS
-import qualified LinearScan.IntSet as LS
 import qualified LinearScan.Interval as LS
 import qualified LinearScan.LiveSets as LS
 import qualified LinearScan.Loops as LS
 import qualified LinearScan.Main as LS
 import qualified LinearScan.Monad as Coq
 import qualified LinearScan.Range as LS
+import qualified LinearScan.Resolve as LS
 import qualified LinearScan.Trace as LS
 import qualified LinearScan.UsePos as LS
 import qualified LinearScan.Verify as LS
@@ -77,7 +77,7 @@ data VarInfo = VarInfo
     }
 
 deriving instance Eq LS.VarKind
-deriving instance Show LS.VarKind
+-- deriving instance Show LS.VarKind
 
 fromVarInfo :: LinearScan.VarInfo -> LS.VarInfo
 fromVarInfo (VarInfo a b c) = LS.Build_VarInfo a b c
@@ -96,11 +96,11 @@ fromVarInfo (VarInfo a b c) = LS.Build_VarInfo a b c
 data OpInfo m op1 op2 = OpInfo
     { opKind      :: op1 -> OpKind
     , opRefs      :: op1 -> [LinearScan.VarInfo]
-    , moveOp      :: PhysReg   -> PhysReg   -> m [op2]
-    , swapOp      :: PhysReg   -> PhysReg   -> m [op2]
-    , saveOp      :: PhysReg   -> Maybe Int -> m [op2]
-    , restoreOp   :: Maybe Int -> PhysReg   -> m [op2]
-    , applyAllocs :: op1 -> [(Int, PhysReg)] -> m [op2]
+    , moveOp      :: PhysReg  -> LS.VarId -> PhysReg   -> m [op2]
+    , swapOp      :: PhysReg  -> LS.VarId -> PhysReg   -> LS.VarId -> m [op2]
+    , saveOp      :: PhysReg  -> LS.VarId -> m [op2]
+    , restoreOp   :: LS.VarId -> PhysReg   -> m [op2]
+    , applyAllocs :: op1 -> [(LS.VarId, PhysReg)] -> m [op2]
     , showOp1     :: op1 -> String
     }
 
@@ -109,9 +109,10 @@ showOp1' :: (op1 -> String)
            -- Interval Id, it's identity, and possible assigned reg
          -> [(Int, Either PhysReg LS.VarId, Maybe PhysReg)]
          -> [(Int, Either PhysReg LS.VarId, Maybe PhysReg)]
+         -> [LS.ResolvingMoveSet]
          -> op1
          -> String
-showOp1' showop pos ins outs o =
+showOp1' showop pos ins outs rms o =
     let showerv (Left r)  = "r" ++ show r
         showerv (Right v) = "v" ++ show v in
     let render Nothing = ""
@@ -123,7 +124,8 @@ showOp1' showop pos ins outs o =
              else "[" ++ show i ++ "]") ++ render reg ++ ">\n" in
     concatMap (marker "End") outs ++
     concatMap (marker "Beg") ins ++
-    show pos ++ ": " ++ showop o ++ "\n"
+    show pos ++ ": " ++ showop o ++ "\n" ++
+    concatMap (\x -> show x ++ "\n") rms
 
 deriving instance Eq OpKind
 deriving instance Show OpKind
@@ -138,40 +140,38 @@ fromOpInfo (OpInfo a b c d e f g h) =
         (\r1 r2 -> U.unsafeCoerce (f r1 r2))
         (\r1 r2 -> U.unsafeCoerce (g r1 r2)) h
 
-type IntervalId = Int
-
 data ScanStateDesc = ScanStateDesc
     { _nextInterval  :: Int
     , intervals      :: [LS.IntervalDesc]
     , fixedIntervals :: [Maybe LS.IntervalDesc]
-    , unhandled      :: [(IntervalId, Int)]
-    , active         :: [(IntervalId, PhysReg)]
-    , inactive       :: [(IntervalId, PhysReg)]
-    , handled        :: [(IntervalId, Maybe PhysReg)]
+    , unhandled      :: IntMap Int
+    , active         :: IntMap PhysReg
+    , inactive       :: IntMap PhysReg
+    , handled        :: IntMap (Maybe PhysReg)
     , allocations    :: IntMap PhysReg
     }
 
-deriving instance Show LS.IntervalDesc
-deriving instance Show LS.RangeDesc
-deriving instance Show LS.UsePos
+-- deriving instance Show LS.IntervalDesc
+-- deriving instance Show LS.RangeDesc
+-- deriving instance Show LS.UsePos
 
 instance Show ScanStateDesc where
     show sd =
         "Unhandled:\n"
             ++ concatMap (\(i, _) -> "  " ++ showInterval i ++ "\n")
-                         (unhandled sd) ++
+                         (M.toList (unhandled sd)) ++
         "Active:\n"
             ++ concatMap (\(i, r) ->
                            "  r" ++ show r ++ showInterval i ++ "\n")
-                         (active sd) ++
+                         (M.toList (active sd)) ++
         "Inactive:\n"
             ++ concatMap (\(i, r) ->
                            "  r" ++ show r ++ showInterval i ++ "\n")
-                         (inactive sd) ++
+                         (M.toList (inactive sd)) ++
         "Handled:\n"
             ++ concatMap (\(i, r) ->
                            "  " ++ showReg r ++ showInterval i ++ "\n")
-                         (handled sd) ++
+                         (M.toList (handled sd)) ++
         "Fixed:\n"
             ++ concatMap (\(reg, mi) ->
                            case mi of
@@ -214,7 +214,8 @@ toScanStateDesc (LS.Build_ScanStateDescSet a b c d e f g) =
                             Just r -> M.insert k r m)
                  M.empty g in
     let xs = L.foldl' (\m (k, r) -> M.insert k r m) rs (e ++ f) in
-    ScanStateDesc a b c d e f g xs
+    ScanStateDesc a b c
+        (M.fromList d) (M.fromList e) (M.fromList f) (M.fromList g) xs
 
 data LoopState = LoopState
     { activeBlocks     :: IntSet
@@ -255,8 +256,8 @@ tracer x = Debug.Trace.trace ("====================\n" ++ x)
 showBlock1 :: (blk1 -> [op1])
            -> LS.BlockId
            -> LS.OpId
-           -> [Int]
-           -> [Int]
+           -> IntSet
+           -> IntSet
            -> (LS.OpId -> [op1] -> String)
            -> blk1
            -> String
@@ -265,10 +266,14 @@ showBlock1 getops bid pos liveIns liveOuts showops b =
     " => IN:" ++ show liveIns ++ " OUT:" ++ show liveOuts ++ "\n" ++
     showops pos (getops b)
 
-showOps1 :: LinearScan.OpInfo accType op1 op2 -> ScanStateDesc -> Int -> [op1]
+showOps1 :: LinearScan.OpInfo accType op1 op2
+         -> ScanStateDesc
+         -> IntMap [LS.ResolvingMoveSet]
+         -> Int
+         -> [op1]
          -> String
-showOps1 _ _ _ [] = ""
-showOps1 oinfo sd pos (o:os) =
+showOps1 _ _ _ _ [] = ""
+showOps1 oinfo sd rms pos (o:os) =
     let here = pos*2+1 in
     let allocs = allocations sd in
     let k idx (bacc, eacc) i =
@@ -293,8 +298,9 @@ showOps1 oinfo sd pos (o:os) =
     -- let (begs', ends') =
     --         LS.vfoldl'_with_index (0 :: Int) r (begs, ends)
     --                               (fixedIntervals sd) in
-    showOp1' (showOp1 oinfo) (pos*2+1) begs ends o
-        ++ showOps1 oinfo sd (pos+1) os
+    showOp1' (showOp1 oinfo) (pos*2+1) begs ends
+        (fromMaybe [] (M.lookup (pos*2+1) rms)) o
+        ++ showOps1 oinfo sd rms (pos+1) os
 
 -- | From the point of view of this library, a basic block is nothing more
 --   than an ordered sequence of operations.
@@ -310,22 +316,24 @@ showBlocks1 :: Monad m
             => LinearScan.BlockInfo m blk1 blk2 op1 op2
             -> LinearScan.OpInfo m op1 op2
             -> ScanStateDesc
-            -> LS.IntMap LS.BlockLiveSets
+            -> IntMap LS.BlockLiveSets
+            -> IntMap [LS.ResolvingMoveSet]
             -> [blk1]
             -> m String
-showBlocks1 binfo oinfo sd ls = go 0
+showBlocks1 binfo oinfo sd ls rms = go 0
   where
     go _ [] = return ""
     go pos (b:bs) = do
         bid <- LinearScan.blockId binfo b
         let (liveIn, liveOut) =
-                 case LS.coq_IntMap_lookup bid ls of
-                     Nothing -> (LS.emptyIntSet, LS.emptyIntSet)
-                     Just s  -> (LS.blockLiveIn s, LS.blockLiveOut s)
+                 case M.lookup bid ls of
+                     Nothing -> (S.empty, S.empty)
+                     Just s  -> (S.fromList (LS.blockLiveIn s),
+                                 S.fromList (LS.blockLiveOut s))
         let allops blk =
                 let (x, y, z) = LinearScan.blockOps binfo blk in
                 x ++ y ++ z
-        (showBlock1 allops bid pos liveIn liveOut (showOps1 oinfo sd) b ++)
+        (showBlock1 allops bid pos liveIn liveOut (showOps1 oinfo sd rms) b ++)
             `liftM` go (pos + length (allops b)) bs
 
 fromBlockInfo :: Monad m
@@ -340,11 +348,12 @@ fromBlockInfo (BlockInfo a b c d e) =
 
 data Details m blk1 blk2 op1 op2 = Details
     { reason          :: Maybe ([LS.SSTrace], LS.FinalStage)
-    , liveSets        :: [(Int, LS.BlockLiveSets)]
+    , liveSets        :: IntMap LS.BlockLiveSets
+    , resolvingMoves  :: IntMap [LS.ResolvingMoveSet]
     , _inputBlocks    :: [blk1]
     , orderedBlocks   :: [blk1]
-    , allocatedBlocks :: Either (LS.OpId, [LS.AllocError]) [blk2]
-    , scanStatePre    :: Maybe ScanStateDesc
+    , allocatedBlocks :: Either (IntMap [LS.AllocError]) [blk2]
+    , _scanStatePre   :: Maybe ScanStateDesc
     , scanStatePost   :: Maybe ScanStateDesc
     , blockInfo       :: LinearScan.BlockInfo m blk1 blk2 op1 op2
     , opInfo          :: LinearScan.OpInfo m op1 op2
@@ -353,31 +362,49 @@ data Details m blk1 blk2 op1 op2 = Details
 
 deriving instance Show LS.AllocError
 
+instance Show LS.ResolvingMoveSet where
+  show (LS.RSMove fr fv tr) =
+      "<Move (r" ++ show fr ++ " v" ++ show fv ++ ") " ++
+           "(r" ++ show tr ++ " v" ++ show fv ++ ")>"
+  show (LS.RSSwap fr fv tr tv) =
+      "<Swap (r" ++ show fr ++ " v" ++ show fv ++ ") " ++
+           "(r" ++ show tr ++ " v" ++ show tv ++ ")>"
+  show (LS.RSSpill fr tv)    =
+      "<Spill (r" ++ show fr ++ " v" ++ show tv ++ ")>"
+  show (LS.RSRestore fv tr)  =
+      "<Restore (r" ++ show tr ++ " v" ++ show fv ++ ")>"
+  show (LS.RSAllocReg fv tr) =
+      "<AllocReg (r" ++ show tr ++ " v" ++ show fv ++ ")>"
+  show (LS.RSFreeReg fr tv)  =
+      "<FreeReg (r" ++ show fr ++ " v" ++ show tv ++ ")>"
+  -- show (LS.RSAllocStack tv)  = "<AllocStack (v" ++ show tv ++ ")>"
+  -- show (LS.RSFreeStack fv)   = "<FreeStack (v" ++ show fv ++ ")>"
+
+-- showResolvingMoves :: IntMap [LS.ResolvingMoveSet] -> String
+-- showResolvingMoves =
+--     M.foldlWithKey' (\acc k mv ->
+--         acc ++ "    " ++ show k ++ " => "
+--             ++ L.intercalate "\n         " (map show mv) ++ "\n") ""
+
 showDetails :: Monad m => Details m blk1 blk2 op1 op2 -> m String
 showDetails err = do
-    pre  <- showPreScanStateDesc (scanStatePre err)
-    post <- showPostScanStateDesc (scanStatePost err)
+    -- pre  <- showScanStateDesc (scanStatePre err)
+    post <- showScanStateDesc (scanStatePost err)
     return $ "Reason: " ++ show (reason err) ++ "\n\n"
-          ++ ">>> ScanState before allocation:\n"
-          ++ pre ++ "\n"
+          -- ++ ">>> ScanState before allocation:\n"
+          -- ++ pre ++ "\n"
           ++ ">>> ScanState after allocation:\n"
           ++ post ++ "\n"
+          -- ++ ">>> ResolvingMoves =\n"
+          -- ++ showResolvingMoves (resolvingMoves err) ++ "\n"
           ++ ">>> " ++ show (loopState err) ++ "\n"
   where
-    showPreScanStateDesc Nothing = return ""
-    showPreScanStateDesc (Just sd) =
-        liftM2 (++)
-            (showBlocks1 (blockInfo err) (opInfo err) sd
-                         (liveSets err) (orderedBlocks err))
-            (return ("\n" ++ show sd))
-
-    -- jww (2015-05-23): Show allocatedBlocks here?
-    showPostScanStateDesc Nothing = return ""
-    showPostScanStateDesc (Just sd) =
-        liftM2 (++)
-            (showBlocks1 (blockInfo err) (opInfo err) sd
-                         (liveSets err) (orderedBlocks err))
-            (return ("\n" ++ show sd))
+    showScanStateDesc Nothing = return ""
+    showScanStateDesc (Just sd) =
+        liftM2 (++) (showBlocks1 (blockInfo err) (opInfo err) sd
+                                 (liveSets err) (resolvingMoves err)
+                                 (orderedBlocks err))
+                    (return ("\n" ++ show sd))
 
 deriving instance Show LS.FinalStage
 deriving instance Show LS.BlockLiveSets
@@ -401,9 +428,11 @@ toDetails :: LS.Details blk1 blk2
           -> LinearScan.BlockInfo m blk1 blk2 op1 op2
           -> LinearScan.OpInfo m op1 op2
           -> Details m blk1 blk2 op1 op2
-toDetails (LS.Build_Details a b c d e f g h) binfo oinfo =
-    Details a b c d e (fmap toScanStateDesc f) (fmap toScanStateDesc g)
-            binfo oinfo (toLoopState h)
+toDetails (LS.Build_Details a b c d e f g h i) binfo oinfo =
+    Details a (M.fromList b) (M.fromList c) d e
+        (either (Left . M.fromList) Right f)
+        (fmap toScanStateDesc g) (fmap toScanStateDesc h)
+        binfo oinfo (toLoopState i)
 
 -- | Transform a list of basic blocks containing variable references, into an
 --   equivalent list where each reference is associated with a register
@@ -433,11 +462,13 @@ allocate maxReg binfo oinfo useVerifier blocks = do
             dets <- showDetails res'
             return $ Left $ tracer dets $ map reasonToStr err
         Nothing -> case allocatedBlocks res' of
-            Left (pos, es)    -> do
+            Left m -> do
                 dets <- showDetails res'
                 return $ Left $ tracer dets $
                     -- jww (2015-07-02): NYI
-                    ["At position " ++ show pos] ++ map show es
+                    concatMap (\(pos, es) ->
+                                ("At position " ++ show pos) : map show es)
+                              (M.toList m)
             Right blks -> return $ Right blks
   where
     reasonToStr r = case r of
