src/Resolve.v
@@ -1,4 +1,5 @@
 Require Import LinearScan.Lib.
+Require Import Hask.Data.Maybe.
 Require Import LinearScan.Graph.
 Require Import LinearScan.UsePos.
 Require Import LinearScan.Interval.
@@ -24,49 +25,185 @@ Context `{mDict : Monad mType}.
 Variable binfo : BlockInfo blockType1 blockType2 opType1 opType2.
 Variable oinfo : OpInfo maxReg opType1 opType2.
 
-Definition RawResolvingMove := (option PhysReg * option PhysReg)%type.
-
 Inductive ResolvingMove :=
-  | Move    of PhysReg & PhysReg
-  | Swap    of PhysReg & PhysReg
-  | Spill   of PhysReg & VarId
-  | Restore of VarId   & PhysReg
-  | Nop.
+  | Move       of PhysReg & VarId & PhysReg
+  | Swap       of PhysReg & VarId & PhysReg & VarId
+  | Spill      of PhysReg & VarId
+  | Restore    of VarId & PhysReg
+  | AllocReg   of VarId & PhysReg
+  | FreeReg    of PhysReg & VarId
+  (* | AllocStack of VarId *)
+  (* | FreeStack  of VarId *)
+.
 
-Definition determineMove vid (x : RawResolvingMove) : ResolvingMove :=
+Inductive ResolvingMoveSet : Set :=
+  | RSMove       of nat & VarId & nat
+  | RSSwap       of nat & VarId & nat & VarId
+  | RSSpill      of nat & VarId
+  | RSRestore    of VarId & nat
+  | RSAllocReg   of VarId & nat
+  | RSFreeReg    of nat & VarId
+  (* | RSAllocStack of VarId *)
+  (* | RSFreeStack  of VarId *)
+.
+
+Definition weakenResolvingMove (x : ResolvingMove) : ResolvingMoveSet :=
   match x with
-  | (Some x, Some y) => Move x y
-  | (Some x, None)   => Spill x vid
-  | (None,   Some y) => Restore vid y
-  | (None,   None)   => Nop
+  | Move       fr fv tr    => RSMove       fr fv tr
+  | Swap       fr fv tr tv => RSSwap       fr fv tr tv
+  | Spill      fr tv       => RSSpill      fr tv
+  | Restore    fv tr       => RSRestore    fv tr
+  | AllocReg   fv tr       => RSAllocReg   fv tr
+  | FreeReg    fr tv       => RSFreeReg    fr tv
+  (* | AllocStack tv          => RSAllocStack tv *)
+  (* | FreeStack  fv          => RSFreeStack  fv *)
   end.
 
-Definition prepareForGraph vid (x : RawResolvingMove) :
-  option (sum_eqType (ordinal_eqType maxReg) nat_eqType) *
-  option (sum_eqType (ordinal_eqType maxReg) nat_eqType) :=
-  match x with
-  | (Some x, Some y) => (Some (inl x), Some (inl y))
-  | (Some x, None)   => (Some (inl x), Some (inr vid))
-  | (None,   Some y) => (Some (inr vid), Some (inl y))
-  | (None,   None)   => (Some (inr vid), Some (inr vid))
+Section EqResolvingMove.
+
+Implicit Type s : ResolvingMove.
+
+Definition eqResolvingMove s1 s2 :=
+  match s1, s2 with
+  | Move fr1 fv1 tr1,     Move fr2 fv2 tr2     =>
+    [&& fr1 == fr2, fv1 == fv2 & tr1 == tr2]
+  | Swap fr1 fv1 tr1 tv1, Swap fr2 fv2 tr2 tv2 =>
+    [&& fr1 == fr2, fv1 == fv2, tr1 == tr2 & tv1 == tv2]
+  | Spill fr1 fv1,        Spill fr2 fv2        =>
+    [&& fr1 == fr2 & fv1 == fv2]
+  | Restore tv1 tr1,      Restore tv2 tr2      =>
+    [&& tv1 == tv2 & tr1 == tr2]
+  | AllocReg fv1 tr1,     AllocReg fv2 tr2     =>
+    [&& fv1 == fv2 & tr1 == tr2]
+  | FreeReg fr1 tv1,      FreeReg fr2 tv2      =>
+    [&& fr1 == fr2 & tv1 == tv2]
+  (* | AllocStack tv1,       AllocStack tv2       => *)
+  (*   tv1 == tv2 *)
+  (* | FreeStack fv1,        FreeStack fv2        => *)
+  (*   fv1 == fv2 *)
+  | _, _ => false
   end.
 
-Definition moveFromGraph
-  (mv : option (sum_eqType (ordinal_eqType maxReg) nat_eqType) *
-        option (sum_eqType (ordinal_eqType maxReg) nat_eqType)) :
-  ResolvingMove :=
-  match mv with
-  | (Some (inl x), Some (inl y)) => Move x y
-  | (Some (inl x), Some (inr y)) => Spill x y
-  | (Some (inr x), Some (inl y)) => Restore x y
-  | _ => Nop
+Lemma eqResolvingMoveP : Equality.axiom eqResolvingMove.
+Proof.
+  move.
+  case=> [fr1 fv1 tr1|fr1 fv1 tr1 tv1|fr1 fv1
+         |tv1 tr1|fv1 tr1|fr1 tv1(* |tv1|fv1 *)];
+  case=> [fr2 fv2 tr2|fr2 fv2 tr2 tv2|fr2 fv2
+         |tv2 tr2|fv2 tr2|fr2 tv2(* |tv2|fv2 *)] /=;
+  try by constructor.
+  - case: (fr1 =P fr2) => [<-|?];
+    case: (fv1 =P fv2) => [<-|?];
+    case: (tr1 =P tr2) => [<-|?];
+    first [ by constructor | by right; case ].
+  - case: (fr1 =P fr2) => [<-|?];
+    case: (fv1 =P fv2) => [<-|?];
+    case: (tr1 =P tr2) => [<-|?];
+    case: (tv1 =P tv2) => [<-|?];
+    first [ by constructor | by right; case ].
+  - case: (fr1 =P fr2) => [<-|?];
+    case: (fv1 =P fv2) => [<-|?];
+    first [ by constructor | by right; case ].
+  - case: (tv1 =P tv2) => [<-|?];
+    case: (tr1 =P tr2) => [<-|?];
+    first [ by constructor | by right; case ].
+  - case: (fv1 =P fv2) => [<-|?];
+    case: (tr1 =P tr2) => [<-|?];
+    first [ by constructor | by right; case ].
+  - case: (fr1 =P fr2) => [<-|?];
+    case: (tv1 =P tv2) => [<-|?];
+    first [ by constructor | by right; case ].
+  (* - case: (tv1 =P tv2) => [<-|?]; *)
+  (*   first [ by constructor | by right; case ]. *)
+  (* - case: (fv1 =P fv2) => [<-|?]; *)
+  (*   first [ by constructor | by right; case ]. *)
+Qed.
+
+Canonical ResolvingMove_eqMixin := EqMixin eqResolvingMoveP.
+Canonical ResolvingMove_eqType :=
+  Eval hnf in EqType ResolvingMove ResolvingMove_eqMixin.
+
+End EqResolvingMove.
+
+Definition ResGraphNode := sum_eqType (ordinal_eqType maxReg) nat_eqType.
+
+Record ResGraphEdge := {
+  resMove  : ResolvingMove;
+  resGhost : bool;
+  resBeg   : option ResGraphNode;
+  resEnd   : option ResGraphNode
+}.
+
+Section EqResGraphEdge.
+
+Implicit Type s : ResGraphEdge.
+
+Definition eqResGraphEdge s1 s2 :=
+  match s1, s2 with
+  | {| resMove  := a1
+     ; resGhost := b1
+     ; resBeg   := c1
+     ; resEnd   := d1
+     |},
+    {| resMove  := a2
+     ; resGhost := b2
+     ; resBeg   := c2
+     ; resEnd   := d2
+     |} =>
+    [&& a1 == a2, b1 == b2, c1 == c2 & d1 == d2]
   end.
 
-Definition determineMoves (moves : IntMap RawResolvingMove) :
-  seq ResolvingMove :=
-  let graph := forFold emptyGraph (IntMap_toList moves) $ fun g mv =>
-                 addEdge (prepareForGraph (fst mv) (snd mv)) g in
-  map moveFromGraph (topsort graph).
+Lemma eqResGraphEdgeP : Equality.axiom eqResGraphEdge.
+Proof.
+  move.
+  case=> [a1 b1 c1 d1].
+  case=> [a2 b2 c2 d2] /=.
+  case: (a1 =P a2) => [<-|?]; last by right; case.
+  case: (b1 =P b2) => [<-|?]; last by right; case.
+  case: (c1 =P c2) => [<-|?]; last by right; case.
+  case: (d1 =P d2) => [<-|?]; last by right; case.
+  by constructor.
+Qed.
+
+Canonical ResGraphEdge_eqMixin := EqMixin eqResGraphEdgeP.
+Canonical ResGraphEdge_eqType :=
+  Eval hnf in EqType ResGraphEdge ResGraphEdge_eqMixin.
+
+End EqResGraphEdge.
+
+Definition determineEdge (x : ResGraphEdge) :
+  option ResGraphNode * option ResGraphNode := (resBeg x, resEnd x).
+
+Definition splitEdge (x : ResGraphEdge) : seq ResGraphEdge :=
+  match resMove x with
+  | Move       fr fv tr    =>
+    [:: {| resMove  := Spill fr fv
+         ; resGhost := false
+         ; resBeg   := resBeg x
+         ; resEnd   := None
+         |}
+     ;  {| resMove  := Restore fv tr
+         ; resGhost := resGhost x
+         ; resBeg   := None
+         ; resEnd   := resEnd x
+         |} ]
+  | Swap       fr fv tr tv =>
+    [:: {| resMove  := Swap tr tv fr fv
+         ; resGhost := resGhost x
+         ; resBeg   := resEnd x
+         ; resEnd   := resBeg x
+         |} ]
+  | Spill      fr fv       => [::] (* jww (2015-07-07): Need to use temp slot *)
+  | Restore    tv tr       => [::]
+  | AllocReg   tv tr       => [::]
+  | FreeReg    fr fv       => [::]
+  (* | AllocStack tv          => [::] *)
+  (* | FreeStack  fv          => [::] *)
+  end.
+
+Definition determineMoves (moves : IntMap ResGraphEdge) : seq ResGraphEdge :=
+  topsort (IntMap_foldl (flip addEdge) (emptyGraph determineEdge) moves)
+          splitEdge.
 
 (* Assuming a transition [from] one point in the procedure [to] another --
    where these two positions may be contiguous, or connected via a branch --
@@ -88,7 +225,7 @@ Definition determineMoves (moves : IntMap RawResolvingMove) :
    mean that the program is assuming the variable is live somehow in a
    register or on the stack. *)
 Definition resolvingMoves (allocs : seq (Allocation maxReg)) (from to : nat) :
-  IntMap RawResolvingMove :=
+  IntMap ResGraphEdge :=
 
   (* First determine all of the variables which are live at [from] *at the end
      of that instruction*, either in registers or on the stack.  Then gather
@@ -96,54 +233,108 @@ Definition resolvingMoves (allocs : seq (Allocation maxReg)) (from to : nat) :
   let liveAtFrom :=
       IntMap_fromList [seq (ivar (intVal i), i) | i <- allocs
                       & ibeg (intVal i) <= from < iend (intVal i)] in
-  let liveAtTo :=
-      IntMap_fromList [seq (ivar (intVal i), i) | i <- allocs
-                      & let int := intVal i in
-                        (ibeg int <= to) &&
-                        (if to == iend int
-                         then if lastUsePos int is Some u
-                              then to <= u
-                              else false
-                         else to < iend int)] in
 
+  (* This function is greatly complicated by the fact that there are
+     zero-length "ephemeral" allocations, where a value is loaded into a
+     register only to make it available as input to the next instruction, but
+     only for that instruction. These are handled by allocating and then
+     immediately freeing the register, so that it lives in the register as
+     "ghost" for that one instruction (see Verify.v). *)
+  let shouldKeep int pos :=
+    if ibeg int <= pos
+    then (if pos == iend int
+          then (if lastUsePos int is Some u
+                then to <= u
+                else false, true (* resGhost *))
+          else (to < iend int, false))
+    else (false, false) in
+
+  let liveAtTo :=
+      IntMap_fromList [seq (ivar (intVal i),
+                            (i, snd (shouldKeep (intVal i) to)))
+                      | i <- allocs & fst (shouldKeep (intVal i) to)] in
+
+  (* We use an [IntMap] here to easily detect via merge which variables are
+     coming into being, and which are being dropped. *)
   IntMap_mergeWithKey
-    (fun vid x y =>
+    (fun vid x yp =>
+       let: (y, ghost) := yp in
        if intReg x == intReg y
-       then None
-       else if match intReg x, intReg y with
-               | None,   Some _ => true (* intervalBeginsWithInput (intVal y) *)
-               | _, _ => true
-               end
-            then Some (intReg x, intReg y)
-            else None)
-    (fun _ => emptyIntMap)
-    (fun _ => emptyIntMap)
+       then if intReg y is Some reg
+            then if ghost
+                 then Some {| resMove  := FreeReg reg vid
+                            ; resGhost := true
+                            ; resBeg   := Some (inl reg)
+                            ; resEnd   := Some (inr vid) |}
+                 else None
+            else None
+       else
+         let mmv :=
+            match intReg x, intReg y with
+            | Some xr, Some yr => Some (Move xr vid yr)
+            | Some xr, None    => Some (Spill xr vid)
+            | None,    Some xr => Some (Restore vid xr)
+            | None,    None    => None
+            end in
+         let anchor x := (inl <$> intReg x) <|> Some (inr vid) in
+         if mmv is Some mv
+         then Some {| resMove  := mv
+                    ; resGhost := ghost
+                    ; resBeg   := anchor x
+                    ; resEnd   := anchor y |}
+         else None)
+
+    (IntMap_foldlWithKey
+       (fun acc vid x =>
+          if intReg x is Some r
+          then IntMap_insert vid
+             {| resMove  := FreeReg r vid
+              ; resGhost := false
+              ; resBeg   := Some (inl r)
+              ; resEnd   := Some (inr vid) |} acc
+          else (* FreeStack vid *) acc) emptyIntMap)
+
+    (IntMap_foldlWithKey
+       (fun acc vid yp =>
+          let: (y, ghost) := yp in
+          if intReg y is Some r
+          then IntMap_insert vid
+             {| resMove  := AllocReg vid r
+              ; resGhost := ghost
+              ; resBeg   := Some (inr vid)
+              ; resEnd   := Some (inl r) |} acc
+          else (* AllocStack vid *) acc) emptyIntMap)
+
     liveAtFrom liveAtTo.
 
-Definition checkBlockBoundary (allocs : seq (Allocation maxReg))
-  bid in_from from to liveIn mappings :=
-  let select acc vid x := if IntSet_member vid liveIn
-                          then (vid, x) :: acc
-                          else acc in
-  let moves := IntMap_foldlWithKey select [::] $
-               resolvingMoves allocs (blockLastOpId from)
-                                     (blockFirstOpId to) in
+Definition BlockMoves : Type :=
+  (Graph ResGraphNode ResGraphEdge_eqType *
+   Graph ResGraphNode ResGraphEdge_eqType).
+
+Definition movesBetween (allocs : seq (Allocation maxReg)) (from to : nat) :
+  seq ResGraphEdge :=
+  IntMap_foldl (flip cons) [::] $ resolvingMoves allocs from to.
+
+Definition applyMappings (bid : BlockId) (mappings : IntMap BlockMoves)
+  (in_from : bool) (moves : seq ResGraphEdge) : IntMap BlockMoves :=
   forFold mappings moves $ fun ms mv =>
     let addToGraphs e xs :=
         let: (gbeg, gend) := xs in
         if in_from
         then (gbeg, addEdge e gend)
         else (addEdge e gbeg, gend) in
-    let f mxs :=
-        addToGraphs (prepareForGraph (fst mv) (snd mv)) $
-          if mxs is Some xs
-          then xs
-          else (emptyGraph, emptyGraph) in
+    let eg := emptyGraph determineEdge in
+    let f mxs := addToGraphs mv $ if mxs is Some xs
+                                  then xs
+                                  else (eg, eg) in
     IntMap_alter (@Some _ \o f) bid ms.
 
-Definition BlockMoves :=
-  (Graph (sum_eqType (ordinal_eqType maxReg) nat_eqType) *
-   Graph (sum_eqType (ordinal_eqType maxReg) nat_eqType))%type.
+Definition checkBlockBoundary (allocs : seq (Allocation maxReg))
+  bid in_from from to (liveIn : IntSet) (mappings : IntMap BlockMoves) :
+  IntMap BlockMoves :=
+  applyMappings bid mappings in_from $
+                movesBetween allocs (blockLastOpId from)
+                                    (blockFirstOpId to).
 
 Definition resolveDataFlow (allocs : seq (Allocation maxReg))
   (blocks : seq blockType1) (liveSets : IntMap BlockLiveSets) :
@@ -173,20 +364,34 @@ Definition resolveDataFlow (allocs : seq (Allocation maxReg))
          resolver.resolve_mappings()
        end for
      end for *)
-  forFoldM emptyIntMap blocks $ fun mappings b =>
+  fmap fst $ forFoldM (emptyIntMap, true) blocks $ fun z b =>
+    let: (mappings, isFirst) := z in
     bid <-- blockId binfo b ;;
     (* jww (2015-01-28): Failure here should be impossible *)
     if IntMap_lookup bid liveSets isn't Some from
-    then pure mappings
+    then pure (mappings, false)
     else
+      let mappings' :=
+        if isFirst
+        then applyMappings bid mappings false $
+                           movesBetween allocs 1 (blockFirstOpId from)
+        else mappings in
       suxs <-- blockSuccessors binfo b ;;
       (* If [in_from] is [true], resolving moves are inserted at the end of
          the [from] block, rather than the beginning of the [to] block. *)
       let in_from := size suxs <= 1 in
-      pure $ forFold mappings suxs $ fun ms s_bid =>
-        (* jww (2015-01-28): Failure here should be impossible *)
-        if IntMap_lookup s_bid liveSets isn't Some to then ms else
-        let key := if in_from then bid else s_bid in
-        checkBlockBoundary allocs key in_from from to (blockLiveIn to) ms.
+      let mappings'' :=
+        if size suxs == 0
+        then
+          applyMappings bid mappings' true $
+                        movesBetween allocs (blockLastOpId from)
+                                            (blockLastOpId from).+2
+        else
+          forFold mappings' suxs $ fun ms s_bid =>
+            (* jww (2015-01-28): Failure here should be impossible *)
+            if IntMap_lookup s_bid liveSets isn't Some to then ms else
+            let key := if in_from then bid else s_bid in
+            checkBlockBoundary allocs key in_from from to (blockLiveIn to) ms in
+      pure (mappings'', false).
 
 End Resolve.
