src/Verify.v
@@ -20,6 +20,8 @@ Variable maxReg : nat.          (* max number of registers *)
 Definition PhysReg := 'I_maxReg.
 
 Variable maxVar : nat.          (* max number of variables *)
+Hypothesis variables_exist : 0 < maxVar.
+
 Variables opType1 opType2 : Set.
 Variables mType : Type -> Type.
 Context `{mDict : Monad mType}.
@@ -32,15 +34,19 @@ Inductive UseVerifier :=
   | VerifyEnabled.
 
 Record RegStateDesc := {
-  rsRegs   : Vec (option 'I_maxVar) maxReg;
-  rsAllocs : Vec (option 'I_maxReg) maxVar;
-  rsStack  : Vec bool maxVar
+  rsRegs        : Vec (option 'I_maxVar) maxReg;
+  rsAllocs      : Vec (option 'I_maxReg) maxVar;
+  rsGhostRegs   : Vec (option 'I_maxVar) maxReg;
+  rsGhostAllocs : Vec (option 'I_maxReg) maxVar;
+  rsStack       : Vec bool maxVar
 }.
 
 Definition newRegStateDesc : RegStateDesc :=
-  {| rsRegs   := vconst None
-   ; rsAllocs := vconst None
-   ; rsStack  := vconst false
+  {| rsRegs        := vconst None
+   ; rsAllocs      := vconst None
+   ; rsGhostRegs   := vconst None
+   ; rsGhostAllocs := vconst None
+   ; rsStack       := vconst false
    |}.
 
 Definition IntSet_to_seq_fin {n : nat} (s : IntSet) :
@@ -55,6 +61,7 @@ Definition keepOnly {A : Type} `(xs : seq 'I_n) :
   Vec (option A) n -> Vec (option A) n :=
   vmap_with_index (fun i x => if i \in xs then x else None).
 
+(* The pattern is: actual, actual, expected *)
 Inductive AllocError :=
   | VarId_OutOfBounds of VarId & nat
   | VarNotAllocated of VarId
@@ -62,31 +69,52 @@ Inductive AllocError :=
   | FreeVarAllocatedToDifferentReg of VarId & nat & nat
   | FreeRegNotAllocatedToVar of nat & VarId
   | VarWithoutAllocation of VarId
-  | VarAllocatedToDifferentReg of VarId & nat & nat
-  | RegNotAllocated of nat
+  | AllocVarAllocatedToDifferentReg of VarId & nat & nat
+  | CheckVarAllocatedToDifferentReg of VarId & nat & nat
+  | MoveRegNotAllocated of nat & nat
+  | SwapRegNotAllocated of nat & nat
+  | SpillRegNotAllocated of nat & nat
   | RegNotAllocatedToVar of nat & VarId
-  | RegAllocatedToDifferentVar of nat & VarId & VarId
+  | CheckRegAllocatedToDifferentVar of nat & VarId & VarId
+  | AllocRegAllocatedToDifferentVar of nat & VarId & VarId
   | RegAlreadyAllocatedTo of nat & VarId
-  | SpillingToWrongSlot of nat & VarId & VarId
+  | SpillToWrongSlot of nat & VarId & VarId
   | BlockWithoutPredecessors of BlockId
   | UnknownPredecessorBlock of BlockId & BlockId
   | ErrorAtBlockEnd of BlockId.
 
-Definition checkAlloc' st (var : 'I_maxVar) (strict : bool) :
+Definition checkAlloc' st (var : 'I_maxVar) (mreg : option 'I_maxReg)
+  (strict : bool) (checkGhosts : bool) :
   option AllocError :=
-  if vnth (rsAllocs st) var isn't Some reg
-  then if strict
-       then Some (VarNotAllocated var)
-       else None
-  else if vnth (rsRegs st) reg isn't Some var'
-       then Some (RegNotAllocatedToVar reg var)
-       else if var == var'
-            then None
-            else Some (RegAllocatedToDifferentVar reg var var').
+  let check regs reg :=
+    let res :=
+      if vnth regs reg isn't Some var'
+      then Some (RegNotAllocatedToVar reg var)
+      else
+        if var == var'
+        then None
+        else Some (CheckRegAllocatedToDifferentVar reg var' var) in
+    if mreg is Some reg'
+    then if reg == reg'
+         then res
+         else Some (CheckVarAllocatedToDifferentReg var reg reg')
+    else res in
+  let go :=
+    if vnth (rsAllocs st) var is Some reg
+    then check (rsRegs st) reg
+    else
+      if strict
+      then Some (VarNotAllocated var)
+      else None in
+  if checkGhosts
+  then if vnth (rsGhostAllocs st) var is Some reg
+       then check (rsGhostRegs st) reg
+       else go
+  else go.
 
 Definition checkLiveness st : seq 'I_maxVar -> seq AllocError :=
   flip (forFold [::]) $ fun acc var =>
-    if checkAlloc' st var false is Some err
+    if checkAlloc' st var None false false is Some err
     then err :: acc
     else acc.
 
@@ -96,43 +124,73 @@ Definition liveRegisters st : seq 'I_maxVar -> seq 'I_maxReg :=
     then reg :: acc
     else acc.
 
+Definition clearGhost (reg : 'I_maxReg) (var : 'I_maxVar)
+  (ghostRegs   : Vec (option 'I_maxVar) maxReg)
+  (ghostAllocs : Vec (option 'I_maxReg) maxVar) :
+  (Vec (option 'I_maxVar) maxReg * Vec (option 'I_maxReg) maxVar) :=
+  (if vnth ghostAllocs var is Some r
+   then vreplace ghostRegs r None
+   else ghostRegs,
+   if vnth ghostRegs reg is Some v
+   then vreplace ghostAllocs v None
+   else ghostAllocs).
+
 Inductive RegState : RegStateDesc -> Prop :=
   | StartState : RegState newRegStateDesc
 
-  | AllocReg st r v :
+  | AllocRegS st r v :
     vnth (rsRegs   st) r == None ->
     vnth (rsAllocs st) v == None ->
     RegState
-      {| rsRegs   := vreplace (rsRegs   st) r (Some v)
-       ; rsAllocs := vreplace (rsAllocs st) v (Some r)
-       ; rsStack  := rsStack st
+      {| rsRegs        := vreplace (rsRegs   st) r (Some v)
+       ; rsAllocs      := vreplace (rsAllocs st) v (Some r)
+       ; rsGhostRegs   := rsGhostRegs   st
+       ; rsGhostAllocs := vreplace (rsGhostAllocs st) v None
+       ; rsStack       := rsStack st
        |}
 
-  | FreeReg st r v :
+  | FreeRegS st r v :
     vnth (rsRegs   st) r == Some v ->
     vnth (rsAllocs st) v == Some r ->
+    let: (gregs, gallocs) :=
+       clearGhost r v (rsGhostRegs st) (rsGhostAllocs st) in
     RegState
-      {| rsRegs   := vreplace (rsRegs   st) r None
-       ; rsAllocs := vreplace (rsAllocs st) v None
-       ; rsStack  := rsStack st
+      {| rsRegs        := vreplace (rsRegs   st) r None
+       ; rsAllocs      := vreplace (rsAllocs st) v None
+       ; rsGhostRegs   := vreplace gregs r (Some v)
+       ; rsGhostAllocs := vreplace gallocs v (Some r)
+       ; rsStack       := rsStack st
        |}
 
-  | AllocStack st v :
+  | ClearGhostsS st :
+    RegState
+      {| rsRegs        := rsRegs st
+       ; rsAllocs      := rsAllocs st
+       ; rsGhostRegs   := vconst None
+       ; rsGhostAllocs := vconst None
+       ; rsStack       := rsStack st
+       |}
+
+  | AllocStackS st v :
     vnth (rsAllocs st) v == None ->
     vnth (rsStack  st) v == false ->
     RegState
-      {| rsRegs   := rsRegs st
-       ; rsAllocs := rsAllocs st
-       ; rsStack  := vreplace (rsStack st) v true
+      {| rsRegs        := rsRegs st
+       ; rsAllocs      := rsAllocs st
+       ; rsGhostRegs   := rsGhostRegs st
+       ; rsGhostAllocs := rsGhostAllocs st
+       ; rsStack       := vreplace (rsStack st) v true
        |}
 
-  | FreeStack st v :
+  | FreeStackS st v :
     vnth (rsAllocs st) v == None ->
     vnth (rsStack  st) v == true ->
     RegState
-      {| rsRegs   := rsRegs st
-       ; rsAllocs := rsAllocs st
-       ; rsStack  := vreplace (rsStack st) v false
+      {| rsRegs        := rsRegs st
+       ; rsAllocs      := rsAllocs st
+       ; rsGhostRegs   := rsGhostRegs st
+       ; rsGhostAllocs := rsGhostAllocs st
+       ; rsStack       := vreplace (rsStack st) v false
        |}.
 
 Definition getRegStateDesc `(st : RegState rd) := rd.
@@ -143,7 +201,8 @@ Arguments packRegState [rd] st /.
 
 Variable A : Type.
 
-Definition BlockExitAllocations := IntMap (seq ('I_maxVar * 'I_maxReg)).
+Definition BlockExitAllocations :=
+  IntMap (seq (('I_maxVar + 'I_maxVar) * 'I_maxReg)).
 
 Record VerifiedSig := {
   verDesc   : RegStateDesc;
@@ -151,6 +210,8 @@ Record VerifiedSig := {
   (* [verBlocks] gives the final allocation state for any blocks; it only
      contains mappings for variables listed in a block's "live out" set. *)
   verBlocks : BlockExitAllocations;
+  verMoves  : IntMap (seq (@ResolvingMove maxReg));
+  verErrors : IntMap (seq AllocError);
   verExt    : A
 }.
 
@@ -158,6 +219,8 @@ Definition newVerifiedSig (i : A) :=
   {| verDesc   := newRegStateDesc
    ; verState  := StartState
    ; verBlocks := emptyIntMap
+   ; verMoves  := emptyIntMap
+   ; verErrors := emptyIntMap
    ; verExt    := i |}.
 
 Definition _verDesc : Getter VerifiedSig RegStateDesc := fun _ _ _ f s =>
@@ -169,6 +232,8 @@ Definition _verState :
     {| verDesc   := x.1
      ; verState  := x.2
      ; verBlocks := verBlocks s
+     ; verMoves  := verMoves s
+     ; verErrors := verErrors s
      ; verExt    := verExt s
      |}) (f (verDesc s; verState s)).
 
@@ -177,78 +242,98 @@ Definition _verBlocks : Lens' VerifiedSig BlockExitAllocations := fun _ _ f s =>
     {| verDesc   := verDesc s
      ; verState  := verState s
      ; verBlocks := x
+     ; verMoves  := verMoves s
+     ; verErrors := verErrors s
      ; verExt    := verExt s
      |}) (f (verBlocks s)).
+
+Definition _verMoves :
+  Lens' VerifiedSig (IntMap (seq (@ResolvingMove maxReg))) := fun _ _ f s =>
+  fmap (fun x =>
+    {| verDesc   := verDesc s
+     ; verState  := verState s
+     ; verBlocks := verBlocks s
+     ; verMoves  := x
+     ; verErrors := verErrors s
+     ; verExt    := verExt s
+     |}) (f (verMoves s)).
+
+Definition _verErrors :
+  Lens' VerifiedSig (IntMap (seq AllocError)) := fun _ _ f s =>
+  fmap (fun x =>
+    {| verDesc   := verDesc s
+     ; verState  := verState s
+     ; verBlocks := verBlocks s
+     ; verMoves  := verMoves s
+     ; verErrors := x
+     ; verExt    := verExt s
+     |}) (f (verErrors s)).
 
 Definition _verExt : Lens' VerifiedSig A := fun _ _ f s =>
   fmap (fun x =>
     {| verDesc   := verDesc s
      ; verState  := verState s
      ; verBlocks := verBlocks s
+     ; verMoves  := verMoves s
+     ; verErrors := verErrors s
      ; verExt    := x
      |}) (f (verExt s)).
 
-(* The [Verified] transformer stack uses [EitherT] to allow sudden exit due to
-   error, otherwise it maintains the current [RegState] plus whatever
-   additional state the user desires. *)
-Definition Verified :=
-  StateT VerifiedSig (EitherT (OpId * seq AllocError) mType).
+Definition Verified := StateT VerifiedSig mType.
 
-Definition _aside {a b : Type} {P : a -> Prop} :
-  Lens' { x : a * b | P (fst x) } b :=
-  fun _ _ f s =>
-    let: exist (x, y) H := s in
-    fmap (fun z => exist _ (x, z) H) (f y).
+Variable pc : OpId.(varReg dst)
 
-Definition runVerified `(m : Verified b) (i : A) :
-  mType ((OpId * seq AllocError) + b) :=
-  fst <$> m (newVerifiedSig i).
+Definition errorsT (errs : seq AllocError) : Verified unit :=
+  _verErrors %= IntMap_insert pc errs.
 
-Variable pc : OpId.
-
-Definition errorsT {a} (errs : seq AllocError) : Verified a :=
-  fun _ => pure $ inl (pc, errs).
-
-Definition errorT {a} (err : AllocError) : Verified a :=
+Definition errorT (err : AllocError) : Verified unit :=
   errorsT [:: err].
 
 Variable useVerifier : UseVerifier.
 
-Definition checkAlloc (var : 'I_maxVar) : Verified unit :=
+Definition checkAlloc (var : 'I_maxVar) (reg : 'I_maxReg) (checkGhosts : bool) :
+  Verified unit :=
   st <-- use _verDesc ;;
-  if checkAlloc' st var (if useVerifier is VerifyEnabled
-                         then true else false) is Some err
+  if checkAlloc' st var (Some reg)
+                 (if useVerifier is VerifyEnabled
+                  then true else false) checkGhosts is Some err
   then errorT err
   else pure tt.
 
+Definition addMove (mv : @ResolvingMove maxReg) : Verified unit :=
+  _verMoves %= IntMap_alter
+    (fun mxs => @Some _ $ if mxs is Some xs
+                          then rcons xs mv
+                          else [:: mv]) pc.
+
 Definition allocReg (reg : 'I_maxReg) (var : 'I_maxVar) : Verified unit :=
+  addMove $ AllocReg var reg ;;
   st <-- use _verDesc ;;
-  a  <-- use _verExt ;;
   decide (vnth (rsRegs st) reg == None)
     (fun H1 =>
        decide (vnth (rsAllocs st) var == None)
-         (fun H2 => _verState .= packRegState (AllocReg H1 H2))
+         (fun H2 => _verState .= packRegState (AllocRegS H1 H2))
          (fun _  =>
             if vnth (rsAllocs st) var is Some r
-            then errorT $ VarAllocatedToDifferentReg var reg r
+            then errorT $ AllocVarAllocatedToDifferentReg var r reg
             else pure tt))
     (fun _  =>
        if vnth (rsRegs st) reg is Some v
        then
          when (v != var) $
-           errorT $ RegAllocatedToDifferentVar reg var v
+           errorT $ AllocRegAllocatedToDifferentVar reg v var
        else pure tt).
 
 Definition freeReg (reg : 'I_maxReg) (var : 'I_maxVar) : Verified unit :=
+  addMove $ FreeReg reg var ;;
   st <-- use _verDesc ;;
-  a  <-- use _verExt ;;
   decide (vnth (rsRegs st) reg == Some var)
     (fun H1 =>
        decide (vnth (rsAllocs st) var == Some reg)
-         (fun H2 => _verState .= packRegState (FreeReg H1 H2))
+         (fun H2 => _verState .= packRegState (FreeRegS H1 H2))
          (fun _  =>
             if vnth (rsAllocs st) var is Some r
-            then errorT $ FreeVarAllocatedToDifferentReg var reg r
+            then errorT $ FreeVarAllocatedToDifferentReg var r reg
             else errorT $ FreeUnallocatedVar var))
     (fun _  => errorT $ FreeRegNotAllocatedToVar reg var).
 
@@ -260,55 +345,101 @@ Lemma size_is0 : forall a (l : seq a), l = nil -> size l == 0.
 Proof. move=> a. by case. Qed.
 
 Definition checkVar (vid : VarId) : Verified 'I_maxVar :=
-  decide (vid < maxVar)
-    (fun H => pure $ Ordinal H)
-    (fun _ => errorT $ VarId_OutOfBounds vid maxVar).
+  if prop (vid < maxVar) is Some H
+  then pure $ Ordinal H
+  else
+    errorT $ VarId_OutOfBounds vid maxVar ;;
+    pure $ Ordinal variables_exist.
 
 Definition verifyBlockBegin (bid : nat) (liveIns : IntSet) (loops : LoopState) :
   Verified unit :=
-  if useVerifier isn't VerifyEnabled then pure tt else
+  if useVerifier is VerifyDisabled then pure tt else
   if IntMap_lookup bid (forwardBranches loops) is Some fwds
-  then forM_ (IntSet_toList fwds) $ fun pred =>
-    exits <-- use _verBlocks ;;
-    if IntMap_lookup pred exits isn't Some allocs
-    then errorT $ UnknownPredecessorBlock bid pred
-    else forM_ (IntSet_toList liveIns) $ fun vid =>
-      var <-- checkVar vid ;;
-      if maybeLookup allocs var isn't Some reg
-      then pure tt (* errorT $ VarWithoutAllocation vid *)
-      else allocReg reg var
+  then
+    forFoldM true (IntSet_toList fwds) (fun isFirst pred =>
+      exits <-- use _verBlocks ;;
+      (if IntMap_lookup pred exits isn't Some allocs
+       then errorT $ UnknownPredecessorBlock bid pred
+       (* else forM_ (IntSet_toList liveIns) $ fun vid => *)
+       (*   var <-- checkVar vid ;; *)
+       (*   if maybeLookup allocs (inr var) is Some reg *)
+       (*   then allocReg reg var *)
+       (*   else *)
+       (*     if maybeLookup allocs (inl var) is Some reg *)
+       (*     then allocReg reg var ;; *)
+       (*          freeReg reg var *)
+       (*     else errorT $ VarWithoutAllocation vid *)
+       else
+         forM_ (IntSet_toList liveIns) (fun vid =>
+           var <-- checkVar vid ;;
+           if maybeLookup allocs (inr var) is Some reg
+           then pure tt
+           else
+             if maybeLookup allocs (inl var) is Some reg
+             then pure tt
+             else errorT $ VarWithoutAllocation vid) ;;
+         when isFirst $
+           forM_ allocs $ fun z =>
+             match z with
+             | (inl var, reg) => allocReg reg var ;;
+                                 freeReg reg var
+             | (inr var, reg) => allocReg reg var
+             end) ;;
+      pure false) ;;
+    pure tt
   else
     if IntSet_size liveIns == 0
     then pure tt
-    else errorT $ BlockWithoutPredecessors bid.
+    else
+      if useVerifier is VerifyEnabledUnitializedOK
+      then pure tt
+      else errorT $ BlockWithoutPredecessors bid.
 
 Definition verifyBlockEnd (bid : nat) (liveOuts : IntSet) : Verified unit :=
-  if useVerifier isn't VerifyEnabled then pure tt else
+  if useVerifier is VerifyDisabled then pure tt else
+  st <-- use _verDesc ;;
+
+  let allocs := vfoldl_with_index
+    (fun var acc mreg =>
+       if mreg is Some reg
+       then (inr var, reg) :: acc
+       else acc) [::] (rsAllocs st) in
+
+  let allocs' := vfoldl_with_index
+    (fun var acc mreg =>
+       if mreg is Some reg
+       then if maybeLookup acc (inr var) is None
+            then if maybeValueLookup acc reg is None
+                 then (inl var, reg) :: acc
+                 else acc
+            else acc
+       else acc) allocs (rsGhostAllocs st) in
+
+  _verBlocks %= IntMap_insert bid allocs' ;;
+
   decide (all (ltn ^~ maxVar) (IntSet_toList liveOuts))
     (fun L =>
        st <-- use _verDesc ;;
        let vars := IntSet_to_seq_fin L in
        if checkLiveness st vars is e :: es
        then errorsT $ ErrorAtBlockEnd bid :: e :: es
-       else
-         _verBlocks %= IntMap_insert bid
-           (forFold [::] vars $ fun acc var =>
-             if vnth (rsAllocs st) var is Some reg
-             then (var, reg) :: acc
-             else acc) ;;
-         (* Clear out all known allocations *)
-         _verState .= packRegState StartState)
+       else pure tt)
     (fun _ =>
        forM_ (IntSet_toList liveOuts) $ fun var =>
          when (maxVar <= var) $
-           errorT $ VarId_OutOfBounds var maxVar).
+           errorT $ VarId_OutOfBounds var maxVar) ;;
 
+  (* Clear out all known allocations *)
+  _verState .= packRegState StartState.
+
+(*
 Definition replaceReg (reg : 'I_maxReg) (var : 'I_maxVar) : Verified unit :=
   st <-- use _verDesc ;;
   (if vnth (rsRegs st) reg is Some v
    then freeReg reg v
    else pure tt) ;;
   allocReg reg var.
+*)
 
 Definition verifyApplyAllocs (op : opType1) (allocs : seq (VarId * PhysReg)) :
   Verified (seq opType2) :=
@@ -334,55 +465,98 @@ Definition verifyApplyAllocs (op : opType1) (allocs : seq (VarId * PhysReg)) :
          else
            var <-- checkVar vid ;;
            match varKind ref with
-           | Input  => checkAlloc var
+           | Input  => checkAlloc var reg true
            | Temp   => pure tt         (* jww (2015-07-04): What to do here? *)
-           | Output => replaceReg reg var
+           | Output => checkAlloc var reg false
            end
        end)
    else pure tt) ;;
 
-  lift $ lift $ applyAllocs oinfo op allocs.
+  (* st <-- use _verDesc ;; *)
+  (* _verState .= packRegState (ClearGhostsS st) ;; *)
 
-Definition verifyResolutions (moves : seq (ResolvingMove maxReg)) :
-  Verified unit :=
-  if useVerifier isn't VerifyEnabled then pure tt else
-  forM_ moves $ fun mv =>
+  lift $ applyAllocs oinfo op allocs.
+
+Definition verifyResolutions (moves : seq (@ResGraphEdge maxReg)) :
+  Verified (seq (ResolvingMove maxReg)) :=
+  if useVerifier is VerifyDisabled
+  then pure $ map (@resMove maxReg) moves else
+  fmap rev $ forFoldM [::] moves $ fun acc mv =>
     st <-- use _verDesc ;;
-    match mv with
-    | Move fromReg toReg =>
+    match resMove mv with
+    | Move fromReg fromVar toReg =>
       if vnth (rsRegs st) fromReg isn't Some fromVar
-      then errorT $ RegNotAllocated fromReg
+      then
+        errorT $ MoveRegNotAllocated fromReg toReg ;;
+        addMove (resMove mv) ;;
+        pure acc
       else
-        freeReg fromReg fromVar ;;
-        allocReg toReg fromVar
+        if fromReg == toReg
+        then pure acc
+        else
+          freeReg fromReg fromVar ;;
+          allocReg toReg fromVar ;;
+          addMove (resMove mv) ;;
+          when (resGhost mv) (freeReg toReg fromVar) ;;
+          pure $ resMove mv :: acc
 
-    | Swap fromReg toReg =>
+    | Swap fromReg fromVar toReg toVar =>
       if vnth (rsRegs st) fromReg isn't Some fromVar
-      then errorT $ RegNotAllocated fromReg
+      then
+        errorT $ SwapRegNotAllocated fromReg toReg ;;
+        addMove (resMove mv) ;;
+        pure acc
       else
         if vnth (rsRegs st) toReg isn't Some toVar
-        then errorT $ RegNotAllocated toReg
+        then
+          errorT $ SwapRegNotAllocated toReg fromReg ;;
+          addMove (resMove mv) ;;
+          pure acc
         else
-          when (fromVar != toVar) $
-            freeReg toReg toVar ;;
-            freeReg fromReg fromVar ;;
-            allocReg toReg fromVar ;;
-            allocReg fromReg toVar
+          if fromVar != toVar
+          then checkAlloc toVar toReg false ;;
+               checkAlloc fromVar fromReg false ;;
+               addMove (resMove mv) ;;
+               pure $ resMove mv :: acc
+          else pure acc
 
     | Spill fromReg toSpillSlot =>
       if vnth (rsRegs st) fromReg isn't Some fromVar
-      then errorT $ RegNotAllocated fromReg
+      then
+        errorT $ SpillRegNotAllocated fromReg toSpillSlot ;;
+        addMove (resMove mv) ;;
+        pure acc
       else
-        freeReg fromReg fromVar ;;
         stackVar <-- checkVar toSpillSlot ;;
-        when (fromVar != stackVar) $
-          errorT $ SpillingToWrongSlot fromReg toSpillSlot fromVar
+        if fromVar != stackVar
+        then
+          errorT $ SpillToWrongSlot fromReg fromVar toSpillSlot ;;
+          addMove (resMove mv) ;;
+          pure acc
+        else
+          addMove (resMove mv) ;;
+          freeReg fromReg fromVar ;;
+          pure $ resMove mv :: acc
 
     | Restore fromSpillSlot toReg =>
       stackVar <-- checkVar fromSpillSlot ;;
-      replaceReg toReg stackVar
+      allocReg toReg stackVar ;;
+      addMove (resMove mv) ;;
+      when (resGhost mv) (freeReg toReg stackVar) ;;
+      pure $ resMove mv :: acc
 
-    | Nop => pure tt
+    | AllocReg toVar toReg =>
+      var <-- checkVar toVar ;;
+      allocReg toReg var ;;
+      when (resGhost mv) (freeReg toReg var) ;;
+      pure acc
+
+    | FreeReg fromReg fromVar =>
+      checkVar fromVar >>= freeReg fromReg ;;
+      pure acc
+
+    (* | AllocStack toVar => pure acc *)
+    (* | FreeStack fromVar => pure acc *)
     end.
 
 End Verify.
@@ -394,12 +568,14 @@ Include LensLaws.
 Variable a b : Type.
 Variable P : a -> Prop.
 
-Program Instance Lens__aside : LensLaws (@_aside a b P).
-
 (* Program Instance Lens__verDesc : GetterLaws (@_verDesc maxReg maxVar a). *)
 Program Instance Lens__verState : LensLaws (@_verState maxReg maxVar a).
 Obligation 2. by case: x. Qed.
 Program Instance Lens__verBlocks : LensLaws (@_verBlocks maxReg maxVar a).
+Obligation 2. by case: x. Qed.
+Program Instance Lens__verMoves : LensLaws (@_verMoves maxReg maxVar a).
+Obligation 2. by case: x. Qed.
+Program Instance Lens__verErrors : LensLaws (@_verErrors maxReg maxVar a).
 Obligation 2. by case: x. Qed.
 Program Instance Lens__verExt : LensLaws (@_verExt maxReg maxVar a).
 Obligation 2. by case: x. Qed.
